possibly simplify live_tile_stride_cells slightly

src/lib/poly/gemm/Kuiper.Poly.GEMM.Copy.Vec.fsti
@@ -48,26 +48,20 @@ let live_tile_stride_cells
   : slprop
 =
   // typeclass constraint not resolved automatically
-  forall+ (idx : natlt (rows*cols) {tid = idx/(chunk et #_ #hvc) % nthr /\ chunk et /?+ idx}).
-    if (idx%cols < cols - chunk et + 1)
-    // this fact about (idx%cols) should be provable here, we add it only to avoid a
-    // hard VC at this point, punting the proof on to the user (where it's
-    // hopefully easier)
-    then live_chunk m (idx/cols) (idx%cols)
-    else emp
- 
-//  // Number of chunks each thread will copy
-//  forall+ (it : natlt (divup (rows*cols) (chunk et * nthr))).
-//    let flat_idx = tid * chunk et + it * nthr * chunk et <: nat in
-//    let i : nat = flat_idx / cols in
-//    let j : nat = flat_idx % cols in
-//    if i < rows
-//       && j < cols - chunk et + 1
-//       // this fact about j should be provable here, we add it only to avoid a
-//       // hard VC at this point, punting the proof on to the user (where it's
-//       // hopefully easier)
-//    then live_chunk m i j
-//    else emp
+  forall+ (idx : natlt (rows*cols) {tid = idx/(chunk et #_ #hvc) % nthr /\ chunk et /?+ idx /\ idx%cols < cols - chunk et + 1}).
+    live_chunk m (idx/cols) (idx%cols)
+  // Number of chunks each thread will copy
+  //forall+ (it : natlt (divup (rows*cols) (chunk et * nthr))).
+  //  let flat_idx = tid * chunk et + it * nthr * chunk et <: nat in
+  //  let i : nat = flat_idx / cols in
+  //  let j : nat = flat_idx % cols in
+  //  if i < rows
+  //     && j < cols - chunk et + 1
+  //     // this fact about j should be provable here, we add it only to avoid a
+  //     // hard VC at this point, punting the proof on to the user (where it's
+  //     // hopefully easier)
+  //  then live_chunk m i j
+  //  else emp
 
 // NB: The scalar constraint is only here so we can use 'zero' as an initializer
 // for a local array... would be gone if we had uninitialized local arrays.
